\section{Appendix}
\subsection{Matrices}
\subsubsection{Transpose, Adjoint and Inverse}
\noindent\begin{align*}
    \mathbf{A}^\mathsf{H}                  & = {(\mathbf{A}^\mathsf{T})}^*                   \\[.75em]
    {({\mathbf{A}}^\mathsf{T})}^\mathsf{T} & = \mathbf{A}                                    \\
    {({\mathbf{A}}^\mathsf{H})}^\mathsf{H} & = \mathbf{A}                                    \\
    {({\mathbf{A}}^{-1})}^{-1}             & = \mathbf{A}                                    \\[.75em]
    {(\lambda\mathbf{A})}^\mathsf{T}       & = \lambda\mathbf{A}^\mathsf{T}                  \\
    {(\lambda\mathbf{A})}^\mathsf{H}       & = \lambda\mathbf{A}^\mathsf{H}                  \\
    {(\lambda\mathbf{A})}^{-1}             & = \lambda^{-1}\mathbf{A}^{-1}                   \\[.75em]
    {(\mathbf{A}+\mathbf{B})}^\mathsf{T}   & = \mathbf{A}^\mathsf{T} + \mathbf{B}^\mathsf{T} \\
    {(\mathbf{A}+\mathbf{B})}^\mathsf{H}   & = \mathbf{A}^\mathsf{H} + \mathbf{B}^\mathsf{H} \\[.75em]
    {(\mathbf{A}\mathbf{B})}^\mathsf{T}    & = \mathbf{B}^\mathsf{T}\mathbf{A}^\mathsf{T}    \\
    {(\mathbf{A}\mathbf{B})}^\mathsf{H}    & = \mathbf{B}^\mathsf{H}\mathbf{A}^\mathsf{H}    \\
    {(\mathbf{A}\mathbf{B})}^{-1}          & = \mathbf{B}^{-1} \mathbf{A}^{-1}               \\[.75em]
    \det(\mathbf{A}^\mathsf{T})            & = \det(\mathbf{A})                              \\
    \det(\mathbf{A}^\mathsf{H})            & = {\det(\mathbf{A})}^*                          \\
    \det(\mathbf{A}^{-1})                  & = {\det(\mathbf{A})}^{-1}                       \\[.75em]
    \mathrm{rank}{(\mathbf{A}^\mathsf{H})} & = \mathrm{rank}(\mathbf{A})                     \\
    \mathrm{rank}{(\mathbf{A}^{-1} )}      & = \mathrm{rank}(\mathbf{A})
\end{align*}

\ptitle{\textbf{A} is symmetric}
\noindent\begin{align*}
    {\mathbf{A}}^\mathsf{T} & = \mathbf{A}   \\
    {\mathbf{A}}^\mathsf{H} & = \mathbf{A}^*
\end{align*}

\ptitle{\textbf{A} is invertible}
\noindent\begin{align*}
    {(\mathbf{A}^\mathsf{T})}^{-1} & = {(\mathbf{A}^{-1})}^\mathsf{T} \\
    {(\mathbf{A}^\mathsf{H})}^{-1} & = {(\mathbf{A}^{-1})}^\mathsf{H}
\end{align*}

\ptitle{\textbf{A} is square}
\noindent\begin{align*}
    \mathrm{eigvals}(\mathbf{A}^\mathsf{T}) & = \mathrm{eigvals}(\mathbf{A})        \\
    \mathrm{eigvals}(\mathbf{A}^\mathsf{H}) & = \mathrm{eigvals}{(\mathbf{A})}^*    \\
    \mathrm{eigvals}(\mathbf{A}^{-1})       & = \mathrm{eigvals}{(\mathbf{A})}^{-1}
\end{align*}

\ptitle{Blocks}
\noindent\begin{equation*}
    \begin{pmatrix}
        A_{11} & \cdots & A_{1n} \\
        \vdots &        & \vdots \\
        A_{m1} & \cdots & A_{mn}
    \end{pmatrix}^\mathsf{H}=
    \begin{pmatrix}
        A_{11}^\mathsf{H} & \cdots & A_{m1}^\mathsf{H} \\
        \vdots            &        & \vdots            \\
        A_{1n}^\mathsf{H} & \cdots & A_{nm}^\mathsf{H}
    \end{pmatrix}
\end{equation*}